\documentclass{article}
\usepackage{amsmath}
\begin{document}

myy2000 \\
p. 219 (1)
$$ f_{jt} = \frac{max[n_{jt}^{up}, n_{jt}^{down}]}{n_{jt}^{up} + n^{down}_{jt}} $$
p. 221 (5)
$$ f_j = \frac{1}{T} 
    \displaystyle\sum_t \frac{max[n_{jt}^{up}, n_{jt}^{down}]}
    {n_{jt}^{up} + n_{jt}^{down}} = 
    \frac{1}{T} \displaystyle\sum_t f_{jt} $$
p. 222 (6)
$$ r_{it} = \alpha_i + \beta_{1,i} r_{m,jt} + 
    \beta_{2,i} [r_{US,t} + e_{jt}] + \varepsilon_{it} $$
p. 225 (7)
$$ R_j^2 = \frac{\sum_i (R_{ij}^2 \times SST_{i,j})}{\sum_i SST_{i,j}} $$
p. 229 (8)
$$ \Psi_j = \log(\frac{f_j - 0.5}{1 - f_j}) $$
p. 229 (9)
$$ \Upsilon_j = \log(\frac{R_j^2}{1 - R_j^2}) $$
p. 246 (16)
$$ R_j^2 = \frac{\sum_{i \in j} R_{i,j}^2 SST_{i,j}}{\sum_{i \in j}SST_{i,j}} =
    \frac{\sum_{i \in j} \frac{\sigma_{m,i,j}^2}{\sigma_{m,i,j}^2 + \sigma_{\epsilon,i,j}^2}
    (\sigma_{m,i,j}^2 + \sigma_{\epsilon,i,j}^2)}
    {\sum_{i \in j} (\sigma_{m,i,j}^2 + \sigma_{\epsilon,i,j}^2)} $$
p. 246 (17)
$$ \Upsilon_j = \log\bigg(\frac{\sigma_{m,j}^2}{\sigma_{\epsilon,j}^2}\bigg) =
    \log(\sigma_{m,j}^2) - \log(\sigma_{\epsilon, j}^2)$$
p. 247 (18)
$$ \log(\sigma_{\epsilon,j}^2) = c_0 + c_1 \log y_i + c_2 \log n_j +
    \boldsymbol{c} \cdot \boldsymbol{x}_j + c_3 g_j + u_j $$
p. 247 (19)
$$ \log(\sigma_{m,j}^2) = c_0 + c_1 \log y_i + c_2 \log n_j +
    \boldsymbol{c} \cdot \boldsymbol{x}_j + c_3 g_j + u_j $$


\begin{equation}
    r_t = a + b_0 \Delta E_t + 
    \sum_\tau b_\tau \Delta E_{t + \tau} + 
    \sum_\tau c_\tau r_{t + \tau} + u_t
\end{equation}

\begin{equation}
    FERC \equiv \sum_\tau b_\tau
\end{equation}

\begin{equation}
    FINC \equiv R_{r_t = a + b_0 \Delta E_t + 
    \sum_\tau b_\tau \Delta E_{t + \tau} + 
    \sum_\tau c_\tau r_{t + \tau} + u_t}^2 - 
    R_{r_t = a + b_0 \Delta E_t + u_t}^2
\end{equation}

haha
\end{document}
